# 6.

If we only consider the original constraint (i.e. the constraints for example $1$ to $N$), the lagrange function with lagrange multipliers $\alpha_n$ and $\beta_n$ is:

$$
\mathcal{L}(b, \mathbf{w}, \mathbf{\xi}, \mathbf{\alpha}, \mathbf{\beta}) = \frac{1}{2} \mathbf{w}^T\mathbf{w} + C \sum_{n=1}^N \xi_n + \sum_{n=1}^N \alpha_n \left(1 - \xi_n - y_n(b + \mathbf{w}^T \mathbf{\Phi(x_n)}) \right) + \sum_{n=1}^N \beta_n (-\xi_n)
$$

For the anchor pseudo-example, we have the constraint:

$$
y_0(\mathbf{w}^T\mathbf{\Phi(x_0)} + b) \geq 1 
$$

Convert into canonical form:

$$
1 - y_0(\mathbf{w}^T \mathbf{\Phi(x_0)} + b) \leq 0
$$

So we can add the term $\gamma_0(1 - y_0(\mathbf{w}^T \mathbf{\Phi(x_0)} + b))$, where $\gamma_0$ is the corresponding lagrange multiplier.

Thus we have the new lagrange function:

$$
\mathcal{L}(b, \mathbf{w}, \mathbf{\xi}, \mathbf{\alpha}, \mathbf{\beta}, \gamma_0) = \frac{1}{2} \mathbf{w}^T\mathbf{w} + C \sum_{n=1}^N \xi_n + \sum_{n=1}^N \alpha_n \left(1 - \xi_n - y_n(b + \mathbf{w}^T \mathbf{\Phi(x_n)}) \right) + \sum_{n=1}^N \beta_n (-\xi_n) + \gamma_0(1 - y_0(\mathbf{w}^T \mathbf{\Phi(x_0)} + b))
$$

For the lagrange dual, we need to solve:

$$
\max_{\alpha, \beta, \gamma_0 \ge 0} \min_{b, \mathbf{w}, \mathbf{\xi}} \mathcal{L}(b, \mathbf{w}, \mathbf{\xi}, \mathbf{\alpha}, \mathbf{\beta}, \gamma_0)
$$

Taking the partial derivative of each variable, we get:

$$
\frac{\partial \mathcal{L}}{\partial b} = 0 \Rightarrow \sum_{n=1}^N \alpha_n y_n + \gamma_0 y_0 = 0
\tag{1}
$$

$$
\frac{\partial \mathcal{L}}{\partial \mathbf{w}} = 0 \Rightarrow \mathbf{w} = \sum_{n=1}^N \alpha_n y_n \mathbf{\Phi(x_n)} + \gamma_0 y_0 \mathbf{\Phi(x_0)}
\tag{2}
$$

$$
\frac{\partial \mathcal{L}}{\partial \xi_n} = 0 \Rightarrow C - \alpha_n - \beta_n = 0 
\tag{3}
$$

Since $\alpha_n \geq 0$ and $\beta_n \geq 0$, we have $ 0 \le \alpha_n \le C$.

From equation $(2)$, we can substitute $\mathbf{w}$ into the Lagrangian and obtain the dual:

$$
\frac{1}{2} \Bigg\| \sum_{n=1}^N \alpha_n y_n \Phi(\mathbf{x}_n) + \gamma_0 y_0 \Phi(\mathbf{x}_0) \Bigg\|^2+ C \sum_{n=1}^N \xi_n + \sum_{n=1}^N \alpha_n \left(1 - \xi_n - y_n(b + \mathbf{w}^T \mathbf{\Phi(x_n)}) \right) + \sum_{n=1}^N \beta_n (-\xi_n) + \gamma_0(1 - y_0(\mathbf{w}^T \mathbf{\Phi(x_0)} + b))
$$

Converting $||\mathbf{w}||^2$ to the proper form, can write:

$$
\begin{split}
||\mathbf{w}||^2 
&= \sum_{n=1}^N \sum_{m=1}^N \alpha_n \alpha_m y_n y_m \mathbf{\Phi(x_n)}^T \mathbf{\Phi(x_m)} + \gamma_0^2 y_0^2 \mathbf{\Phi(x_0)}^T \mathbf{\Phi(x_0)} + 2 \gamma_0 y_0 \sum_{n=1}^N \alpha_n y_n \mathbf{\Phi(x_n)}^T\mathbf{\Phi(x_0)} \\
&= \sum_{n=1}^N \sum_{m=1}^N \alpha_n \alpha_m y_n y_m K(x_n, x_m) + \gamma_0^2 y_0^2 K(x_0, x_0) + 2 \gamma_0 y_0 \sum_{n=1}^N \alpha_n y_n K(x_n, x_0)
\end{split}
$$

Plug in back to the dual, we get:

$$
\frac{1}{2}\sum_{n=1}^N \sum_{m=1}^N \alpha_n \alpha_m y_n y_m K(x_n, x_m) + \frac{1}{2}\gamma_0^2 y_0^2 K(x_0, x_0) + \gamma_0 y_0 \sum_{n=1}^N \alpha_n y_n K(x_n, x_0)+ C \sum_{n=1}^N \xi_n + \sum_{n=1}^N \alpha_n \left(1 - \xi_n - y_n(b + \mathbf{w}^T \mathbf{\Phi(x_n)}) \right) + \sum_{n=1}^N \beta_n (-\xi_n) + \gamma_0(1 - y_0(\mathbf{w}^T \mathbf{\Phi(x_0)} + b))
$$

Expand the terms and we get:

$$
\frac{1}{2}\sum_{n=1}^N \sum_{m=1}^N \alpha_n \alpha_m y_n y_m K(x_n, x_m) + \frac{1}{2}\gamma_0^2 y_0^2 K(x_0, x_0) + \gamma_0 y_0 \sum_{n=1}^N \alpha_n y_n K(x_n, x_0)+C \sum_{n=1}^N \xi_n + \sum_{n=1}^N \alpha_n - \sum_{n=1}^N \alpha_n \xi_n - \sum_{n=1}^N \alpha_n y_n b - \sum_{n=1}^N \alpha_n y_n \mathbf{w}^T \mathbf{\Phi(x_n)} - \sum_{n=1}^N \beta_n \xi_n + \gamma_0 - \gamma_0 y_0 \mathbf{w}^T \mathbf{\Phi(x_0)} - \gamma_0 y_0 b
$$

From equation $(1)$, we have:

$$
\sum_{n=1}^N \alpha_n y_n + \gamma_0 y_0 = 0 \Rightarrow -(\sum_{n=1}^N \alpha_n y_n + \gamma_0 y_0)b = 0
$$

And from equation $(3)$, we have:

$$
(C - \alpha_n - \beta_n)\sum_{n=1}^N \xi_n= 0 
$$

The Largrangian is simplified to:

$$
\frac{1}{2}\sum_{n=1}^N \sum_{m=1}^N \alpha_n \alpha_m y_n y_m K(x_n, x_m) + \frac{1}{2}\gamma_0^2 y_0^2 K(x_0, x_0) + \gamma_0 y_0 \sum_{n=1}^N \alpha_n y_n K(x_n, x_0) + \sum_{n=1}^N \alpha_n  - \sum_{n=1}^N \alpha_n y_n \mathbf{w}^T \mathbf{\Phi(x_n)}  + \gamma_0 - \gamma_0 y_0 \mathbf{w}^T \mathbf{\Phi(x_0)} 
$$

Observe that the 2 terms that contain $\mathbf{w}$ can also be expanded as:

$$
\begin{split}
- \sum_{n=1}^N \alpha_n y_n \mathbf{w}^T \mathbf{\Phi(x_n)}  
&= - \sum_{n=1}^N \alpha_n y_n \left( \sum_{m=1}^N \alpha_m y_m \mathbf{\Phi(x_m)} + \gamma_0 y_0 \mathbf{\Phi(x_0)} \right)^T \mathbf{\Phi(x_n)} \\
&= - \sum_{n=1}^N \sum_{m=1}^N \alpha_n \alpha_m y_n y_m \mathbf{\Phi(x_m)}^T \mathbf{\Phi(x_n)} - \sum_{n=1}^N \alpha_n y_n \gamma_0 y_0 \mathbf{\Phi(x_0)}^T \mathbf{\Phi(x_n)} \\
&= - \sum_{n=1}^N \sum_{m=1}^N \alpha_n \alpha_m y_n y_m K(x_n, x_m) - \sum_{n=1}^N \alpha_n y_n \gamma_0 y_0 K(x_0, x_n)
\end{split}
$$

And:

$$
\begin{split}
- \gamma_0 y_0 \mathbf{w}^T \mathbf{\Phi(x_0)} 
&= - \gamma_0 y_0 \left( \sum_{n=1}^N \alpha_n y_n \mathbf{\Phi(x_n)} + \gamma_0 y_0 \mathbf{\Phi(x_0)} \right)^T \mathbf{\Phi(x_0)} \\
&= - \gamma_0 y_0 \sum_{n=1}^N \alpha_n y_n K(x_n, x_0) - \gamma_0^2 y_0^2 K(x_0, x_0)
\end{split}
$$

Again, plug into the previous simplified Lagrangian, we get:

$$
-\frac{1}{2}\sum_{n=1}^N \sum_{m=1}^N \alpha_n \alpha_m y_n y_m K(x_n, x_m) - \frac{1}{2}\gamma_0^2 y_0^2 K(x_0, x_0) - \gamma_0 y_0 \sum_{n=1}^N \alpha_n y_n K(x_n, x_0) + \sum_{n=1}^N \alpha_n  + \gamma_0 
$$


From the problem description, we knew that $y_0 = -1$ and other $y_n = +1$, so we have:

$$
-\frac{1}{2}\sum_{n=1}^N \sum_{m=1}^N \alpha_n \alpha_m K(x_n, x_m) - \frac{1}{2}\gamma_0^2 K(x_0, x_0) + \gamma_0 \sum_{n=1}^N \alpha_n K(x_n, x_0) + \sum_{n=1}^N \alpha_n  + \gamma_0 
$$

In order to use the QP solver, we first need to convert the above maximization problem into a minimization problem:

$$
\min_{\mathbf{\alpha}, \gamma_0 \ge 0} \frac{1}{2}\sum_{n=1}^N \sum_{m=1}^N \alpha_n \alpha_m K(x_n, x_m) + \frac{1}{2}\gamma_0^2 K(x_0, x_0) - \gamma_0 \sum_{n=1}^N \alpha_n K(x_n, x_0) - \sum_{n=1}^N \alpha_n  - \gamma_0 
$$

Then, we can further use the fact that $\mathbf{x_0} = \mathbf{0}$, so the terms including $K(x_0, x_0)$ and $K(x_n, x_0)$ will be 0, and we will have:

$$
\min_{\mathbf{\alpha}, \gamma_0 \ge 0} \frac{1}{2}\sum_{n=1}^N \sum_{m=1}^N \alpha_n \alpha_m K(x_n, x_m) - \sum_{n=1}^N \alpha_n  - \gamma_0 
$$

Then, consider the stationary condition for $\gamma_0$:

$$
\frac{\partial}{\partial \gamma_0} \left[ \frac{1}{2}\sum_{n=1}^N \sum_{m=1}^N \alpha_n \alpha_m K(x_n, x_m) - \sum_{n=1}^N \alpha_n  - \gamma_0 \right] = 0
$$

We found that $\gamma_0 = 0$.

## Unused

The constraints can also be transformed into:

$$
\sum_{n=1}^N \alpha_n - \gamma_0 = 0 \Rightarrow \mathbf{A} \mathbf{u} = b \qquad \text{
where } \mathbf{A} = \begin{bmatrix}
-1 & 1 & 1 & \cdots & 1 \\
\end{bmatrix}, \ b = 0
$$

Taking summation over $(6)$:

$$
\begin{split}
&\sum_{n=1}^N C - \sum_{n=1}^N \alpha_n - \sum_{n=1}^N \beta_n = 0 \\
\Rightarrow & \ C N - \sum_{n=1}^N \alpha_n - \sum_{n=1}^N \beta_n = 0 \\
\Rightarrow & \  \sum_{n=1}^N \alpha_n = -\sum_{n=1}^N \beta_n + C N 
\end{split}
$$

$$
G \mathbf{u} = \begin{bmatrix}
-1 & 0 & 0 & \cdots & 0 \\
0 & 1 & 0 & \cdots & 0 \\
\vdots & \vdots & \vdots & \ddots & \vdots \\
0 & \cdots & 1 & \cdots & 0 \\
0 & 0 & 0 & -1 \cdots & 0 \\
\vdots & \vdots & \vdots & \ddots & \vdots \\
0 & 0 & 0 & \cdots & -1 \\
\end{bmatrix}
\begin{bmatrix}
\gamma_0 \\
\alpha_1 \\
\alpha_2 \\
\vdots \\
\alpha_N \\
\end{bmatrix} \ge \begin{bmatrix}
CN \\
0 \\
0 \\
\vdots \\
0 \\
\end{bmatrix}
$$
