# 8.

We need to show that $K(x, x') = \mathrm{exp}(2 \cos(x - x') - 2)$ is a valid kernel.

By the definition of a valid kernel, it should be a symmetric and positive semidefinite function, so it is equivalent to show that $\mathbf{K}$ is a valid (i.e. symmetric and positive semidefinite) Gram matrix, where $\mathbf{K}$ is defined as follows:

$$
\mathbf{K} = 
\begin{bmatrix}
K(x_1, x_1) & K(x_1, x_2) & \cdots & K(x_1, x_N) \\
K(x_2, x_1) & K(x_2, x_2) & \cdots & K(x_2, x_N) \\
\vdots & \vdots & \ddots & \vdots \\
K(x_N, x_1) & K(x_N, x_2) & \cdots & K(x_N, x_N)
\end{bmatrix}
$$

To prove the symmetric property, we need to show that for arbitrary $x_i, x_j, \quad K(x_i, x_j) = K(x_j, x_i)$.

Plug in to the definition, and using the property $\cos(x) = \cos(-x)$, we have:

$$
K(x_i, x_j) = \mathrm{exp}(2 \cos(x_i - x_j) - 2) = \mathrm{exp}(2 \cos(x_j - x_i) - 2) = K(x_j, x_i)
$$

Thus, $K(x_i, x_j) = K(x_j, x_i)$ holds.

To prove the positive semidefinite property, we need to show that for arbitrary $\mathbf{z} \in \mathbb{R}^N$, $\mathbf{z}^\top \mathbf{K} \mathbf{z} \ge 0$.

Let $\mathbf{z} = \begin{bmatrix} z_1 & z_2 & \cdots & z_N \end{bmatrix}^\top$, then we have:

$$
\mathbf{z}^\top \mathbf{K} \mathbf{z} = \sum_{i=1}^N \sum_{j=1}^N z_i z_j K(x_i, x_j)
$$

Substitute the definition of $K(x_i, x_j)$, we have:

$$
\begin{split}
\mathbf{z}^\top \mathbf{K} \mathbf{z} 
&= \sum_{i=1}^N \sum_{j=1}^N z_i z_j \mathrm{exp}(2 \cos(x_i - x_j) - 2) \\
&= e^{-2} \sum_{i=1}^N \sum_{j=1}^N z_i z_j \mathrm{exp}(2 \cos(x_i - x_j))  \\
\end{split}
$$

Since $e^{-2} > 0$, we only need to show that:

$$
\sum_{i=1}^N \sum_{j=1}^N z_i z_j \mathrm{exp}(2 \cos(x_i - x_j)) \ge 0
$$

This is equivalent to:

$$
\begin{split}
\sum_{i=1}^N \sum_{j=1}^N z_i z_j \mathrm{exp}(2 (\cos x_i \cos x_j + \sin x_i \sin x_j))
\end{split}
$$

If we define the vectors:

$$
\mathbf{v}_i = \begin{bmatrix} \cos x_i \\ \sin x_i \end{bmatrix}, \quad \mathbf{v}_j = \begin{bmatrix} \cos x_j \\ \sin x_j \end{bmatrix}
$$

Then the above equation can be written as:

$$
\sum_{i=1}^N \sum_{j=1}^N z_i z_j \mathrm{exp}(2 \mathbf{v}_i^\top \mathbf{v}_j)
$$

We further define the matrix $\mathbf{V}$ with:

$$
\mathbf{V}_{ij} = \mathrm{exp}(2 \mathbf{v}_i^\top \mathbf{v}_j)
$$

We can easily see that $\mathbf{V}$ is a symmetric matrix, and since $\mathrm{exp}(2 \mathbf{v}_i^\top \mathbf{v}_j)$ is a positive definite function of the inner product $\mathbf{v}_i^\top \mathbf{v}_j$, $\mathbf{V}$ is a positive (semi)definite matrix.

And we can rewrite the above equation:

$$
\mathbf{z}^\top \mathbf{K} \mathbf{z} = e^{-2}\mathbf{z}^\top \mathbf{V} \mathbf{z}
$$

Since $\mathbf{V}$ is a positive semidefinite matrix, $e^{-2}\mathbf{z}^\top \mathbf{V} \mathbf{z} \ge 0$ holds for arbitrary $\mathbf{z} \in \mathbb{R}^N$.

Thus, $\mathbf{z}^\top \mathbf{K} \mathbf{z} \ge 0$ holds for arbitrary $\mathbf{z} \in \mathbb{R}^N$, and $\mathbf{K}$ is also a positive semidefinite matrix.

Therefore, we have shown that $K(x, x')$ is a valid kernel.